Working on the proofs of bdds

src/BDD.v
@@ -42,49 +42,121 @@ Fixpoint assoc {A B} (eq: A -> A ->  bool) x l : option B :=
 Module Inner. 
   Require Import FMapPositive FMapAVL OrderedTypeAlt.
   Module PMap := PositiveMap.
+
+  (** Rather painful proof of the fact that nodes form an ordered type *)
   Module N <: OrderedTypeAlt.
     Definition t := node.    
-    
+    Require Import Compare. 
     Definition compare (x y : t) := 
-      let '(l1,v1,r1) := x in 
-      let '(l2,v2,r2) := y in 
-        match expr_compare l1 l2 with
-            | Eq => match expr_compare r1 r2 with
-                     | Eq => match NPeano.Nat.compare v1 v2 with
-                                | Eq => Eq
-                                | c => c
-                   end
-            | c => c
-        end
-    | c => c
-         end.
+      lex  (expr_compare (snd x) (snd y)) 
+           (
+             (fun (x: expr * var) (y : expr * var) => 
+                let (r1,v1) := x in 
+                let (r2,v2) := y in 
+                lex (expr_compare r1 r2) (NPeano.Nat.compare v1 v2)) (fst x) (fst y)).
 
-    Lemma compare_sym :
-      forall x y, ( compare y x) = CompOpp (compare x y).
-    Admitted.
-    Lemma compare_trans :
-      forall c x y z, (compare x y) = c -> (compare y z) = c -> (compare x z) = c.
-    Admitted.
+        
+    Lemma expr_compare_sym x y : expr_compare x y = CompOpp (expr_compare y x). 
+    Proof. 
+      unfold expr_compare; destruct x; destruct y; simpl; trivial.  
+      apply Pos.compare_antisym. 
+    Qed. 
+
+    Lemma nat_compare_sym x y : NPeano.Nat.compare x y = CompOpp (NPeano.Nat.compare y x). 
+    Proof.
+      unfold NPeano.Nat.compare. 
+      revert y; induction x. simpl. destruct y; reflexivity. 
+      intros. simpl. destruct y. reflexivity.
+      rewrite nat_compare_S. auto. 
+    Qed.
+
+    Lemma expr_compare_trans c x y z: expr_compare x y = c -> expr_compare y z = c -> expr_compare x z = c.
+    Proof.  
+      unfold expr_compare; destruct x; destruct y; destruct z; simpl; trivial || (try (intros; subst; discriminate)). 
+      destruct c. 
+      intros; rewrite Pos.compare_eq_iff in * |- *. congruence. 
+      intros; rewrite Pos.compare_lt_iff in * |- *. zify.  omega.
+      intros; rewrite Pos.compare_gt_iff in * |- *. zify.  omega.
+    Qed.     
+
+    (* Library issue: compare the two proofs of these lemmas... *)
+    Lemma nat_compare_trans c x y z: NPeano.Nat.compare x y = c -> NPeano.Nat.compare y z = c -> NPeano.Nat.compare x z = c. 
+    Proof. 
+      destruct c; intros; zify. 
+      intros; rewrite nat_compare_eq_iff in * |- *. congruence. 
+      intros; rewrite <- nat_compare_lt in * |- *. zify.  omega.
+      intros; rewrite <- nat_compare_gt in * |- *. zify.  omega.
+    Qed. 
+
+    Hint Resolve expr_compare_trans expr_compare_sym nat_compare_trans nat_compare_sym. 
+    
+    Lemma compare_sym x y :compare y x = CompOpp (compare x y).
+    Proof. 
+      intros. 
+      destruct x as [[l1 v1] r1]; destruct y as [ [l2 v2] r2]; simpl. 
+      apply lex_sym; eauto. 
+      intros [? ?] [? ?]. apply lex_sym; eauto.  
+    Qed.
+
+    
+    Lemma compare_trans c x y z : (compare x y) = c -> (compare y z) = c -> (compare x z) = c.
+    Proof. 
+      apply lex_trans; eauto. 
+      clear. intros c [? ?] [? ?] [? ?].  apply lex_trans; eauto. 
+    Qed. 
   End N.
   Module NO := OrderedType_from_Alt(N).
   
+
   Module NMap := FMapAVL.Make (NO).
   Notation pmap := PMap.t.
   Notation nmap := NMap.t.
+  
+  (** We are now ready to start speaking about BDDs  *)
   Record BDD :=
     {
       tmap : pmap node;
-      hmap : nmap positive;
+      hmap : nmap positive; 
       next : positive
     }. 
 
+  Definition low b (x:expr) : option expr :=
+    match x with 
+      | N x => 
+        match PMap.find x (tmap b) with
+          | Some (y,v,z) => Some y
+          | _ => None
+        end
+      | _ => None end.
+
+  Definition high b (x:expr) :=
+    match x with 
+      | N x => 
+        match PMap.find x (tmap b) with
+          | Some (y,v,z) => Some y
+          | _ => None
+        end
+      | _ => None end.
+
+
+  Definition order (b: BDD) x y :=
+    low b x = Some y \/ high b x = Some y. 
+  
+  Definition wf (b:BDD) := well_founded (order b).
+  
   Definition empty :=
     {|
       tmap := PMap.empty _;
       hmap := NMap.empty _;
       next := 1
-    |}.
-         
+    |}.         
+
+  Lemma wf_empty : wf empty. 
+  Proof.
+    intro x. apply Acc_intro. intros y o. 
+    red in o; destruct o; unfold low, high, empty in H; simpl in H;
+    destruct y; try rewrite PMap.gempty in H; discriminate.
+  Qed.
 
   Definition mk_node bdd (l : expr) (v: var) (h : expr) :=
     if expr_eqb l  h then (l,bdd)
@@ -98,142 +170,218 @@ Module Inner.
                                    next := (u + 1)%positive |} in
                       (N u, bdd)
        end. 
+  
+  Section lex. 
+    Context {A B: Type}. 
+    Variable leA : A -> A -> Prop.
+    Variable leB : B -> B -> Prop.
+    Hypothesis HA : well_founded leA.
+    Hypothesis HB : well_founded leB. 
+    
+    Inductive lex : A * B -> A * B -> Prop := 
+    | left_lex :
+        forall (x x' :A) (y y':B),
+          leA x x' -> lex (x,y) (x',y')
+    | right_lex :
+        forall (x:A) (y y':B),
+          leB y y' -> lex (x,y) (x,y'). 
 
-  Fixpoint andb bdd depth (a b : expr) : option (expr * BDD) :=
-    match depth with 
-      | 0 => None
-      | S depth => 
-          match a,b with 
-            | F, _ => Some (F, bdd)
-            | _, F => Some (F, bdd)
-            | T, x => Some (x, bdd)
-            | x, T => Some (x, bdd)
-            | N na, N nb => 
-                do na <- PMap.find na (tmap bdd);
-                do nb <- PMap.find nb (tmap bdd);
-                match na,nb with 
-                  | (l1,v1,h1),(l2,v2,h2) =>
-                      match NPeano.Nat.compare v1  v2 with 
-                          | Eq =>
-                              do  x ,bdd  <- andb bdd depth l1 l2;
-                              do  y, bdd <- andb bdd depth h1 h2;
-                              Some (mk_node bdd x v1 y)
-                          | Lt =>
-                              do x, bdd <- andb bdd depth l1 b;
-                              do y, bdd <- andb bdd depth h1 b;
-                              Some (mk_node bdd x v1 y)
-                          | _ => 
-                              do x, bdd <- andb bdd depth a l2;
-                              do y, bdd <- andb bdd depth a h2;
-                              Some (mk_node bdd x v2 y)
-                end
+    Lemma lex_wf : well_founded lex. 
+    Proof. 
+    Admitted.
+  End lex. 
+
+  Definition porder bdd : expr * expr -> expr * expr -> Prop := lex (order bdd) (order bdd).
+
+  Section operations.
+
+    Fixpoint eval bdd depth env (a: expr) : option bool :=
+      match depth with 
+        | 0 => None
+        | S depth =>
+          match a with 
+            | T => Some true
+            | F => Some false
+            | N n =>    
+              (        
+              do x <- PMap.find n (tmap bdd);
+              match x with 
+                | (l,v,h) => 
+                  (
+                    do b <- List.nth_error env v;
+                    if (b: bool) 
+                    then eval bdd depth env h
+                    else eval bdd depth env l)              
+              end
+              )
           end
-    end
-       end.
+      end. 
 
-  Fixpoint orb bdd depth (a b : expr) : option (expr * BDD) :=
-    match depth with 
-      | 0 => None
-      | S depth => 
+    Require Import Program.Wf.                  
+
+    Program Fixpoint andb (bdd: BDD) (ab : expr * expr) {wf (porder bdd) ab} : option (expr * BDD) :=
+      match ab with 
+        | (F, _) => Some (F, bdd)
+        | (_, F) => Some (F, bdd)
+        | (T, x) => Some (x, bdd)
+        | (x, T) => Some (x, bdd)
+        | (N na, N nb) => 
+          let a := N na in 
+          let b := N nb in 
+          do na <- PMap.find na (tmap bdd);
+          do nb <- PMap.find nb (tmap bdd);
+            let '(l1,v1,h1) := na in 
+            let '(l2,v2,h2) := nb in 
+            match NPeano.Nat.compare v1  v2 with 
+              | Eq =>
+                do x, bdd <- andb bdd (l1,l2);
+                do y, bdd <- andb bdd (h1,h2);
+                  Some (mk_node bdd x v1 y)
+              | Lt =>
+                  do x, bdd <- andb bdd (l1,b);
+                  do y, bdd <- andb bdd (h1,b);
+                  Some (mk_node bdd x v1 y)
+                | _ => 
+                  do x, bdd <- andb bdd (a,l2);
+                  do y, bdd <- andb bdd (a,h2);
+                  Some (mk_node bdd x v2 y)
+                       
+            end
+      end.
+                  Next Obligation. 
+  End operations.
+  
+  Lemma and_correct bdd n env a b x y ab bdd' :
+    eval bdd n env a = Some x ->
+    eval bdd n env b = Some y ->
+    andb bdd n a b = Some (ab, bdd') ->
+    eval bdd' n env ab = Some (x && y)%bool.
+  Proof.
+     Ltac t := 
+      repeat match goal with 
+               | H : Some _ = Some _ |- _ => injection H; clear H; intros ?
+             end.
+    induction n; intros Ha Hb Hab. 
+    - simpl in *.  discriminate. 
+    - simpl eval in *. 
+      destruct a; destruct b; simpl in Hab; t; intros; subst; f_equal.
+      * auto. 
+      * rewrite Bool.andb_comm. reflexivity. 
+      * rewrite Bool.andb_comm. simpl.  auto. 
+      * invert_do Ha; invert_do Hb. rewrite EQ, EQ1 in Hab. simpl in Hab. 
+        destruct x1 as [[l1 v1] h1]. 
+        destruct x0 as [[l0 v0] h0].       
+        invert_do EQ0; invert_do EQ2.
+        destruct x0; destruct x1. 
+      auto. auto. auto.
+
+ 
+invert_do Hb. rewrite EQ.  simpl. auto. 
+      repeat match goal with 
+          H: (do _ <- _ ; _ = Some _) |- _ => invert_do H
+      end. 
+      + t. exists F. simpl. exists bdd. subst. simpl. intuition. 
+      + t. destruct b. 
+        * t. subst. exists F. exists bdd. simpl; intuition. 
+        * t. subst. exists T. exists bdd; simpl; intuition.
+        *  simpl. exists (N p); exists (bdd). intuition. subst. simpl. apply Hb. 
+      + destruct b;t; subst; simpl. 
+        * exists F; exists bdd. intuition. destruct x; reflexivity.  
+        * exists (N p); exists bdd. intuition. Require Import Bool. rewrite andb_comm. simpl. apply Ha. 
+        * invert_do Ha.  invert_do Hb. rewrite EQ1, EQ.  simpl. 
+          destruct x0; destruct p1; destruct x1. destruct p1.
+          destruct (NPeano.Nat.compare n0 n1). 
+          simpl. invert_do EQ0.  invert_do EQ2. simpl. 
+          
+      Ltac simpl. 
+      
+    Fixpoint orb depth (a b : expr) : option (expr * BDD) :=
+      match depth with 
+        | 0 => None
+        | S depth => 
           match a,b with 
-            | F, x => Some (x, bdd)
-            | x, F => Some (x, bdd)
-            | T, _ => Some (T, bdd)
-            | _, T => Some (T, bdd)
-            | N na, N nb => 
-                do na <- PMap.find na (tmap bdd);
-                do nb <- PMap.find nb (tmap bdd);
-                match na,nb with 
-                  | (l1,v1,h1),(l2,v2,h2) =>
-                      match NPeano.Nat.compare v1  v2 with 
-                          | Eq =>
-                              do x, bdd <- orb bdd depth l1 l2;
-                              do y, bdd <- orb bdd depth h1 h2;
-                              Some (mk_node bdd x v1 y)
-                          | Lt =>
-                              do x, bdd <- orb bdd depth l1 b;
-                              do y, bdd <- orb bdd depth h1 b;
-                              Some (mk_node bdd x v1 y)
-                          | _ => 
-                              do x, bdd <- orb bdd depth a l2;
-                              do y, bdd <- orb bdd depth a h2;
-                              Some (mk_node bdd x v2 y)
+          | F, x => Some (x, bdd)
+          | x, F => Some (x, bdd)
+          | T, _ => Some (T, bdd)
+          | _, T => Some (T, bdd)
+          | N na, N nb => 
+            do na <- PMap.find na (tmap bdd);
+            do nb <- PMap.find nb (tmap bdd);
+            match na,nb with 
+              | (l1,v1,h1),(l2,v2,h2) =>
+                match NPeano.Nat.compare v1  v2 with 
+                  | Eq =>
+                    do x, bdd <- orb depth l1 l2;
+                    do y, bdd <- orb depth h1 h2;
+                      Some (mk_node bdd x v1 y)
+                  | Lt =>
+                    do x, bdd <- orb depth l1 b;
+                    do y, bdd <- orb depth h1 b;
+                    Some (mk_node bdd x v1 y)
+                  | _ => 
+                    do x, bdd <- orb depth a l2;
+                    do y, bdd <- orb depth a h2;
+                    Some (mk_node bdd x v2 y)
                 end
+            end
           end
-    end
-       end.
-
-
-
+      end.
+  
+  
+  
   Fixpoint negb bdd depth (a : expr) : option (expr * BDD) :=
     match depth with 
       | 0 => None
       | S depth => 
-          match a with 
-            | F => Some (T, bdd)
-            | T => Some (F, bdd)
-            | N na => 
-                do na <- PMap.find na (tmap bdd);
-                match na with 
-                  | (l,v,h) =>
-                              do x, bdd <- negb bdd depth l;
-                              do y, bdd <- negb bdd depth h;
-                              Some (mk_node bdd x v y)
-                end
-          end
+        match a with 
+          | F => Some (T, bdd)
+          | T => Some (F, bdd)
+          | N na => 
+            do na <- PMap.find na (tmap bdd);
+              match na with 
+                | (l,v,h) =>
+                  do x, bdd <- negb bdd depth l;
+                    do y, bdd <- negb bdd depth h;
+                    Some (mk_node bdd x v y)
+              end
+        end
     end.
-
+  
   Fixpoint xorb bdd depth (a b : expr) : option (expr * BDD) :=
     match depth with 
       | 0 => None
       | S depth => 
-          match a,b with 
-            | F, x => Some (x, bdd)
-            | x, F => Some (x, bdd)
-            | T, x => negb bdd depth x (* is this depth enough ?? *)
-            | x, T => negb bdd depth x (* is this depth enough ?? *)
-            | N na, N nb => 
-                do na <- PMap.find na (tmap bdd);
-                do nb <- PMap.find nb (tmap bdd);
-                match na,nb with 
-                  | (l1,v1,h1),(l2,v2,h2) =>
-                      match NPeano.Nat.compare v1  v2 with 
-                          | Eq =>
-                              do x, bdd <- xorb bdd depth l1 l2;
-                              do y, bdd <- xorb bdd depth h1 h2;
-                              Some (mk_node bdd x v1 y)
-                          | Lt =>
-                              do x, bdd <- xorb bdd depth l1 b;
-                              do y, bdd <- xorb bdd depth h1 b;
-                              Some (mk_node bdd x v1 y)
-                          | _ => 
-                              do x, bdd <- xorb bdd depth a l2;
-                              do y, bdd <- xorb bdd depth a h2;
-                              Some (mk_node bdd x v2 y)
-                end
-          end
-    end
-       end.
-
+        match a,b with 
+          | F, x => Some (x, bdd)
+          | x, F => Some (x, bdd)
+          | T, x => negb bdd depth x (* is this depth enough ?? *)
+          | x, T => negb bdd depth x (* is this depth enough ?? *)
+          | N na, N nb => 
+            do na <- PMap.find na (tmap bdd);
+              do nb <- PMap.find nb (tmap bdd);
+              match na,nb with 
+                | (l1,v1,h1),(l2,v2,h2) =>
+                  match NPeano.Nat.compare v1  v2 with 
+                    | Eq =>
+                      do x, bdd <- xorb bdd depth l1 l2;
+                        do y, bdd <- xorb bdd depth h1 h2;
+                        Some (mk_node bdd x v1 y)
+                    | Lt =>
+                      do x, bdd <- xorb bdd depth l1 b;
+                        do y, bdd <- xorb bdd depth h1 b;
+                        Some (mk_node bdd x v1 y)
+                    | _ => 
+                      do x, bdd <- xorb bdd depth a l2;
+                        do y, bdd <- xorb bdd depth a h2;
+                        Some (mk_node bdd x v2 y)
+                  end
+              end
+        end
+    end.
+  
   Definition var bdd x :=
     mk_node bdd F x T. 
 
-  Fixpoint eval bdd depth env (a: expr) : option bool :=
-    match depth with 
-      | 0 => None
-      | S depth => match a with 
-                      | T => Some true
-                      | F => Some false
-                      | N n => do x <- PMap.find n (tmap bdd);
-                          match x with 
-                            | (l,v,h) => 
-                                do b <- List.nth_error env v;
-                                if (b: bool) then eval bdd depth env h
-                                else eval bdd depth env l
-                          end
-                  end
-    end. 
-          
 End Inner.
 
 Record BDD := 
